Gnosis/VectorMath.lean
@@ -15,4 +15,29 @@ def cross (v1 v2 : Vector3) : Vector3 :=
    v1.z * v2.x - v1.x * v2.z,
    v1.x * v2.y - v1.y * v2.x⟩
 
+def add (v1 v2 : Vector3) : Vector3 :=
+  ⟨v1.x + v2.x, v1.y + v2.y, v1.z + v2.z⟩
+
+def sub (v1 v2 : Vector3) : Vector3 :=
+  ⟨v1.x - v2.x, v1.y - v2.y, v1.z - v2.z⟩
+
+def neg (v : Vector3) : Vector3 :=
+  ⟨-v.x, -v.y, -v.z⟩
+
+instance : Add Vector3 := ⟨add⟩
+instance : Sub Vector3 := ⟨sub⟩
+instance : Neg Vector3 := ⟨neg⟩
+
+@[simp] theorem add_x (u v : Vector3) : (u + v).x = u.x + v.x := rfl
+@[simp] theorem add_y (u v : Vector3) : (u + v).y = u.y + v.y := rfl
+@[simp] theorem add_z (u v : Vector3) : (u + v).z = u.z + v.z := rfl
+
+@[simp] theorem sub_x (u v : Vector3) : (u - v).x = u.x - v.x := rfl
+@[simp] theorem sub_y (u v : Vector3) : (u - v).y = u.y - v.y := rfl
+@[simp] theorem sub_z (u v : Vector3) : (u - v).z = u.z - v.z := rfl
+
+@[simp] theorem neg_x (u : Vector3) : (-u).x = -u.x := rfl
+@[simp] theorem neg_y (u : Vector3) : (-u).y = -u.y := rfl
+@[simp] theorem neg_z (u : Vector3) : (-u).z = -u.z := rfl
+
 end Gnosis.VectorMath
